some computations in montgomery space

code/kyber2/impl/Impl.Kyber2.Arithmetic.Sums.fst
@@ -12,6 +12,10 @@ open FStar.HyperStack.All
 open FStar.HyperStack
 open FStar.HyperStack.ST
 
+open FStar.Mul
+open FStar.Math.Lemmas
+open Spec.Powtwo.Lemmas
+open Spec.Kyber2.Lemmas
 module ST = FStar.HyperStack.ST
 module Buf = Lib.Buffer
 module Seq = Lib.Sequence
@@ -49,6 +53,58 @@ let sum_n_montgomery #n l output =
       Lib.Arithmetic.Sums.sum_n_simple_lemma2 #Spec.Kyber2.Group.t #Spec.Kyber2.Group.monoid_plus_t (Seq.sub (Seq.map MGroup.to_t h.[|l|]) 0 (v i + 1));
       eq_intro (Seq.sub (Seq.map MGroup.to_t h.[|l|]) 0 (v i)) (Seq.sub (Seq.sub (Seq.map MGroup.to_t h.[|l|]) 0 (v i + 1)) 0 (v i));
       output.(size 0) <- MGroup.plus_m (output.(size 0)) l.(i));
+  let h1 = ST.get () in
+  eq_intro (Seq.sub (Seq.map MGroup.to_t h1.[|l|]) 0 (v n)) (Seq.map MGroup.to_t h1.[|l|])
+
+#reset-options "--z3rlimit 500 --max_fuel 1 --max_ifuel 1"
+val sum_n_montgommery_no_plus_m_inner:
+  #n:size_t{v n < pow2 (params_logr-1)}
+  -> h_:mem
+  -> l:lbuffer (MGroup.montgomery_t) n
+  -> output:lbuffer (x:int32{- params_q * pow2 (params_logr-1) <= sint_v x /\ sint_v x < params_q * pow2 (params_logr -1)}) (size 1)
+  -> i:size_t{0 <= v i /\ v i < v n}
+  -> Stack unit (requires fun h -> (live h l /\ live h output /\ Buf.disjoint l output /\ (sint_v h.[|output|].[0] >= - params_q * (v i)) /\ (sint_v h.[|output|].[0] <= params_q * (v i)) /\ MGroup.int32_to_t (h.[|output|].[0]) == Lib.Arithmetic.Sums.sum_n #Spec.Kyber2.Group.t #Spec.Kyber2.Group.monoid_plus_t (Seq.sub (Seq.map MGroup.to_t h.[|l|]) 0 (v i)) /\ modifies1 output h_ h)) (ensures fun h0 _ h1 -> (live h1 l /\ live h1 output /\ Buf.disjoint l output /\ (sint_v h1.[|output|].[0] >= - params_q * (v i + 1)) /\ (sint_v h1.[|output|].[0] <= params_q * (v i + 1)) /\ MGroup.int32_to_t (h1.[|output|].[0]) == Lib.Arithmetic.Sums.sum_n #Spec.Kyber2.Group.t #Spec.Kyber2.Group.monoid_plus_t (Seq.sub (Seq.map MGroup.to_t h1.[|l|]) 0 (v i + 1)) /\ modifies1 output h_ h1))
+
+#reset-options "--z3rlimit 1000 --max_fuel 1 --max_ifuel 1 --query_stats"
+
+let cast_range a t : Lemma (requires range a t) (ensures a @%. t = a) =
+  pow2_le_compat (bits t) (bits t -1);
+  pow2_double_mult (bits t - 1);
+  cancel_mul_div (pow2 (bits t - 1)) 2;
+  assert(a < modulus t);
+  if (a>=0) then modulo_lemma a (modulus t)
+  else begin
+    pow2_double_sum (bits t - 1);
+    assert(pow2 (bits t - 1) <= a + modulus t);
+    modulo_lemma (a + modulus t) (modulus t);
+    lemma_mod_plus a 1 (modulus t)
+    end
+
+let sum_n_montgommery_no_plus_m_inner #n h0 l output i =
+  let h = ST.get () in
+  Lib.Arithmetic.Sums.sum_n_simple_lemma2 #Spec.Kyber2.Group.t #Spec.Kyber2.Group.monoid_plus_t (Seq.sub (Seq.map MGroup.to_t h.[|l|]) 0 (v i + 1));
+  eq_intro (Seq.sub (Seq.map MGroup.to_t h.[|l|]) 0 (v i)) (Seq.sub (Seq.sub (Seq.map MGroup.to_t h.[|l|]) 0 (v i + 1)) 0 (v i));
+  let k:(x:int32{- params_q * v i <= v x /\ v x <= params_q * v i}) = output.(0ul) in
+  assert( v k + v h.[|l|].[v i] <= params_q * (v i + 1) /\ - params_q * (v i + 1) <= v k + v h.[|l|].[v i]);
+  assert(range (v k + v h.[|l|].[v i]) S32);
+  FStar.Math.Lemmas.lemma_mult_lt_left params_q (v i + 1) (pow2 (params_logr-1));
+  let li:(y:MGroup.montgomery_t{range (v k + v y) S32}) = l.(i) in
+  assert_norm(range (v li) S32);
+  cast_range (v li) S32;
+  MGroup.plus_lemma_int32_2 k li (k +! to_i32 li);
+  assert(MGroup.int32_to_t (k +! to_i32 li) == Group.plus_t (MGroup.int32_to_t k) (MGroup.to_t li));
+  output.(0ul) <- k +! to_i32 li
+
+let sum_n_montgomery_no_plus_m #n l output =
+  let h0 = ST.get () in
+  output.(size 0) <- i32 0;
+  assert_norm(MGroup.int32_to_t (i32 0) == Group.zero_t);
+  assert_norm (0 <= params_q * 0 /\ 0 >= - params_q * 0);
+  Lib.Arithmetic.Sums.sum_n_zero_elements_is_id #Spec.Kyber2.Group.t #Spec.Kyber2.Group.monoid_plus_t (Seq.sub (Seq.map MGroup.to_t h0.[|l|]) 0 0);
+  Lib.Loops.for (size 0) n
+    (fun h i ->
+      (live h l /\ live h output /\ Buf.disjoint l output /\ (sint_v h.[|output|].[0] >= - params_q * i) /\ (sint_v h.[|output|].[0] <= params_q * i) /\ MGroup.int32_to_t (h.[|output|].[0]) == Lib.Arithmetic.Sums.sum_n #Spec.Kyber2.Group.t #Spec.Kyber2.Group.monoid_plus_t (Seq.sub (Seq.map MGroup.to_t h.[|l|]) 0 i) /\ modifies1 output h0 h))
+    (fun i -> sum_n_montgommery_no_plus_m_inner h0 l output i);
   let h1 = ST.get () in
   eq_intro (Seq.sub (Seq.map MGroup.to_t h1.[|l|]) 0 (v n)) (Seq.map MGroup.to_t h1.[|l|])
 
