code/kyber2/impl/Impl.Kyber2.GroupMontgomery.fst
@@ -7,6 +7,8 @@ open Lib.ModularArithmetic.Lemmas
 open FStar.Mul
 open Spec.Kyber2.Params
 open Spec.Kyber2.Reduce
+open Spec.Powtwo.Lemmas
+open Spec.Kyber2.Lemmas
 
 module Group = Impl.Kyber2.Group
 module MGroup = Spec.Kyber2.GroupMontgomery
@@ -20,16 +22,44 @@ let zero_m : montgomery_t = MGroup.zero_m
 inline_for_extraction
 let one_m : montgomery_t = MGroup.one_m
 
-#reset-options "--z3rlimit 100 --max_fuel 1 --max_ifuel 1 --using_facts_from '* -FStar.Seq'"
+#reset-options "--z3rlimit 500 --max_fuel 1 --max_ifuel 1 --using_facts_from '* -FStar.Seq'"
 
 let from_t (x:Group.t) : Pure montgomery_t (requires True) (ensures fun r -> r == MGroup.from_t x) =
   montgomery_reduce_int32 ((to_i32 x) *! (i32 params_mont2))
 
-#reset-options "--z3rlimit 100 --max_fuel 1 --max_ifuel 1 --using_facts_from '* -FStar.Seq'"
+let from_cbd (x:uint16{0 <= uint_v x /\ uint_v x < 19* params_q}) : Pure montgomery_t (requires True) (ensures fun r -> sint_v r % params_q == sint_v (MGroup.from_t (SpecGroup.uint16_to_t x)) % params_q) =
+  assert_norm(19 * params_q * params_mont2 < params_q * pow2 15);
+  assert_norm(19 * params_q * params_mont2 < pow2 31);
+  FStar.Math.Lemmas.lemma_mult_le_right params_mont2 (uint_v x) (19*params_q);
+  FStar.Math.Lemmas.lemma_mult_le_right params_mont2 0 (uint_v x);
+  FStar.Math.Lemmas.modulo_lemma (uint_v x % params_q) params_q;
+  let r2 () : GTot montgomery_t = MGroup.from_t (Group.uint16_to_t x) in
+  assert((sint_v (r2 ()) * pow2 params_logr) % params_q = (SpecGroup.v (Group.uint16_to_t x) * params_mont2) % params_q);
+  FStar.Math.Lemmas.lemma_mod_mul_distr_l (SpecGroup.v (Group.uint16_to_t x)) params_mont2 params_q;
+  FStar.Math.Lemmas.lemma_mod_mul_distr_l (uint_v x) params_mont2 params_q;
+  assert((sint_v (r2 ()) * pow2 params_logr) % params_q = (uint_v x * params_mont2) % params_q);
+  let r () : GTot montgomery_t = montgomery_reduce_int32 ((to_i32 x) *! (i32 params_mont2)) in
+  assert((sint_v (r ()) * pow2 params_logr) % params_q = (uint_v x * params_mont2) % params_q);
+  MGroup.lemma_equality1 (sint_v (r ())) (sint_v (r2 ()));
+  montgomery_reduce_int32 ((to_i32 x) *! (i32 params_mont2))
+
+#reset-options "--z3rlimit 500 --max_fuel 1 --max_ifuel 1 --using_facts_from '* -FStar.Seq'"
 
 
 let to_t (x:montgomery_t) : Pure Group.t (requires True) (ensures fun r -> r == MGroup.to_t #r (from_t r)) =
   let mr = montgomery_reduce_int32 (to_i32 x) in
+  csubq_int16 (mr +! i16 params_q)
+
+let int16_to_t (x:int16) : Pure Group.t (requires True) (ensures fun r -> r == MGroup.to_t #r (from_t r)) =
+  FStar.Math.Lemmas.pow2_lt_compat 31 15;
+  assert_norm(range (sint_v x) S32);
+  let mr = montgomery_reduce_int32 (to_i32 x) in
+  csubq_int16 (mr +! i16 params_q)
+
+let int32_to_t (x:int32) : Pure Group.t (requires (- params_q * pow2 (params_logr-1) <= sint_v x /\ sint_v x < params_q * pow2 (params_logr -1))) (ensures fun r -> r == MGroup.to_t #r (from_t r)) =
+  FStar.Math.Lemmas.pow2_lt_compat 31 15;
+  assert_norm(range (sint_v x) S32);
+  let mr = montgomery_reduce_int32 x in
   csubq_int16 (mr +! i16 params_q)
 
 let to_t_lemma (x:montgomery_t) : Lemma (ensures (sint_v x % params_q = (SpecGroup.v (to_t x) * pow2 params_logr) % params_q /\ to_t x == MGroup.to_t #(to_t x) x)) =
@@ -40,6 +70,31 @@ let to_t_lemma (x:montgomery_t) : Lemma (ensures (sint_v x % params_q = (SpecGro
   lemma_mod_plus (sint_v mr) 1 params_q;
   MGroup.lemma_equality3 (sint_v r) (sint_v x)
 
+let from_cbd_to_t_lemma (x:uint16{0 <= uint_v x /\ uint_v x < 19* params_q}) : Lemma (to_t (from_cbd x) == SpecGroup.uint16_to_t x) =
+  to_t_lemma (from_cbd x);
+  MGroup.lemma_equality1 (SpecGroup.v (to_t (from_cbd x))) (SpecGroup.v (SpecGroup.uint16_to_t x));
+  FStar.Math.Lemmas.modulo_lemma (SpecGroup.v (to_t (from_cbd x))) params_q;
+  FStar.Math.Lemmas.modulo_lemma (SpecGroup.v (to_t (SpecGroup.uint16_to_t x))) params_q
+
+let int16_to_t_lemma (x:int16) : Lemma (ensures (sint_v x % params_q = (SpecGroup.v (int16_to_t x) * pow2 params_logr) % params_q)) =
+  FStar.Math.Lemmas.pow2_lt_compat 31 15;
+  assert_norm(sint_v x @%. S32 == sint_v x);
+  let mr = montgomery_reduce_int32 (to_i32 x) in
+  let r = int16_to_t x in
+  assert((sint_v mr * pow2 params_logr) % params_q = sint_v x % params_q);
+  MGroup.lemma_equality3 (sint_v mr) (sint_v x);
+  lemma_mod_plus (sint_v mr) 1 params_q;
+  MGroup.lemma_equality3 (sint_v r) (sint_v x)
+
+let int32_to_t_lemma (x:int32) : Lemma (requires (- params_q * pow2 (params_logr-1) <= sint_v x /\ sint_v x < params_q * pow2 (params_logr -1))) (ensures (sint_v x % params_q = (SpecGroup.v (int32_to_t x) * pow2 params_logr) % params_q)) =
+  FStar.Math.Lemmas.pow2_lt_compat 31 15;
+  assert_norm(sint_v x @%. S32 == sint_v x);
+  let mr = montgomery_reduce_int32 (to_i32 x) in
+  let r = int32_to_t x in
+  assert((sint_v mr * pow2 params_logr) % params_q = sint_v x % params_q);
+  MGroup.lemma_equality3 (sint_v mr) (sint_v x);
+  lemma_mod_plus (sint_v mr) 1 params_q;
+  MGroup.lemma_equality3 (sint_v r) (sint_v x)
 
 #reset-options "--z3rlimit 100 --max_fuel 0 --max_ifuel 0 --using_facts_from '* -FStar.Seq' --query_stats"
 
@@ -60,19 +115,85 @@ let plus_m (x:montgomery_t) (y:montgomery_t) : Pure montgomery_t (requires True)
   SpecGroup.plus_lemma_t (to_t x) (to_t y);
   barrett_reduce_int16 (x +! y)
 
+let plus_lemma_int32 (x:int32) (y:int32) (z:int32) : Lemma (requires (range (sint_v x + sint_v y) S32 /\ - params_q * pow2 (params_logr-1) <= sint_v x /\ sint_v x < params_q * pow2 (params_logr -1)) /\ (- params_q * pow2 (params_logr-1) <= sint_v y /\ sint_v y < params_q * pow2 (params_logr -1)) /\ (- params_q * pow2 (params_logr-1) <= sint_v x + sint_v y /\ sint_v x + sint_v y < params_q * pow2 (params_logr -1)) /\ sint_v z == sint_v x + sint_v y) (ensures (int32_to_t z == Group.plus_t (int32_to_t x) (int32_to_t y))) =
+  modulo_distributivity (sint_v x) (sint_v y) params_q;
+  int32_to_t_lemma z;
+  int32_to_t_lemma x;
+  int32_to_t_lemma y;
+  modulo_distributivity (SpecGroup.v (int32_to_t x) * pow2 params_logr) (SpecGroup.v (int32_to_t y) * pow2 params_logr) params_q;
+  assert((SpecGroup.v (int32_to_t z) * pow2 params_logr) % params_q = ((SpecGroup.v (int32_to_t x) * pow2 params_logr) + (SpecGroup.v (int32_to_t y) * pow2 params_logr)) % params_q);
+  distributivity_add_left (SpecGroup.v (int32_to_t x)) (SpecGroup.v (int32_to_t y)) (pow2 params_logr);
+  MGroup.lemma_equality1 (SpecGroup.v (int32_to_t z)) (SpecGroup.v (int32_to_t x) + SpecGroup.v (int32_to_t y));
+  modulo_lemma (SpecGroup.v (int32_to_t z)) params_q;
+  SpecGroup.plus_lemma_t (int32_to_t x) (int32_to_t y)
+
+let plus_lemma_int16 (x:int16) (y:int16) (z:int16): Lemma (requires (range (sint_v x + sint_v y) S16 /\ sint_v z == sint_v x + sint_v y)) (ensures (int16_to_t (x +! y) == Group.plus_t (int16_to_t x) (int16_to_t y))) =
+  modulo_distributivity (sint_v x) (sint_v y) params_q;
+  int16_to_t_lemma z;
+  int16_to_t_lemma x;
+  int16_to_t_lemma y;
+  modulo_distributivity (SpecGroup.v (int16_to_t x) * pow2 params_logr) (SpecGroup.v (int16_to_t y) * pow2 params_logr) params_q;
+  assert((SpecGroup.v (int16_to_t z) * pow2 params_logr) % params_q = ((SpecGroup.v (int16_to_t x) * pow2 params_logr) + (SpecGroup.v (int16_to_t y) * pow2 params_logr)) % params_q);
+  distributivity_add_left (SpecGroup.v (int16_to_t x)) (SpecGroup.v (int16_to_t y)) (pow2 params_logr);
+  MGroup.lemma_equality1 (SpecGroup.v (int16_to_t z)) (SpecGroup.v (int16_to_t x) + SpecGroup.v (int16_to_t y));
+  modulo_lemma (SpecGroup.v (int16_to_t z)) params_q;
+  SpecGroup.plus_lemma_t (int16_to_t x) (int16_to_t y)
+
+let plus_lemma_int16_2 (x:int16) (y:montgomery_t) (z:int16): Lemma (requires (range (sint_v x + sint_v y) S16 /\ sint_v z == sint_v x + sint_v y)) (ensures (int16_to_t (x +! y) == Group.plus_t (int16_to_t x) (to_t y))) = plus_lemma_int16 x y z
+
+let plus_lemma_int32_2 (x:int32) (y:montgomery_t) (z:int32) : Lemma (requires (range (sint_v x + sint_v y) S32 /\ - params_q * pow2 (params_logr-1) <= sint_v x /\ sint_v x < params_q * pow2 (params_logr -1)) /\ (- params_q * pow2 (params_logr-1) <= sint_v x + sint_v y /\ sint_v x + sint_v y < params_q * pow2 (params_logr -1) /\ sint_v z == sint_v x + sint_v y)) (ensures (int32_to_t (x +! to_i32 y) == Group.plus_t (int32_to_t x) (to_t y))) = plus_lemma_int32 x (to_i32 y) z
+
 #reset-options "--z3rlimit 2000 --max_fuel 1 --max_ifuel 1 --using_facts_from '* -FStar.Seq'"
 
+let mul_range_lemma_m (x:int16{sint_v x > - pow2 15}) (y:montgomery_t) : Lemma (range (sint_v x * sint_v y) S32 /\  - params_q * pow2 (params_logr-1) <= sint_v x * sint_v y /\ sint_v x * sint_v y < params_q * pow2 (params_logr -1) ) =
+  if (sint_v x >= 0) then begin
+    lemma_mult_le_left (sint_v x) (sint_v y) (params_q);
+    lemma_mult_le_left (sint_v x) (- params_q) (sint_v y);
+    assert(sint_v x * (- params_q) <= sint_v x * sint_v y /\ sint_v x * sint_v y <= sint_v x * params_q);
+    swap_neg_mul (sint_v x) params_q;
+    lemma_mult_le_right (params_q) (- pow2 15) (- sint_v x);
+    lemma_mult_le_right (params_q) (sint_v x) (pow2 15 -1);
+    assert_norm(params_q * pow2 15 < pow2 31);
+    assert(range (sint_v x * sint_v y) S32)
+    end
+  else begin
+    lemma_mult_le_left (- sint_v x) (- sint_v y) (params_q);
+    lemma_mult_le_left (- sint_v x) (- params_q) (sint_v y);
+    assert(- sint_v x * (- params_q) <= sint_v x * sint_v y /\ sint_v x * sint_v y <= - sint_v x * params_q);
+    swap_neg_mul (- sint_v x) (params_q);
+    lemma_mult_le_right (params_q) (- pow2 15) (- sint_v x);
+    lemma_mult_le_right (params_q) ( - sint_v x) (pow2 15 - 1);
+    assert_norm(params_q * pow2 15 < pow2 31);
+    assert(range (sint_v x * sint_v y) S32)
+    end
+
+let mul_range_lemma (x:int16) (y:int16) : Lemma (range (sint_v x * sint_v y) S32) =
+  if (sint_v x >= 0) then begin
+    lemma_mult_le_left (sint_v x) (sint_v y) (pow2 15);
+    lemma_mult_le_left (sint_v x) (- pow2 15) (sint_v y);
+    assert(sint_v x * (- pow2 15) <= sint_v x * sint_v y /\ sint_v x * sint_v y <= sint_v x * pow2 15);
+    swap_neg_mul (sint_v x) (pow2 15);
+    lemma_mult_le_right (pow2 15) (- pow2 15) (- sint_v x);
+    lemma_mult_le_right (pow2 15) (sint_v x) (pow2 15);
+    pow2_plus 15 15;
+    pow2_lt_compat 31 30;
+    assert(range (sint_v x * sint_v y) S32)
+    end
+  else begin
+    lemma_mult_le_left (- sint_v x) (- sint_v y) (pow2 15);
+    lemma_mult_le_left (- sint_v x) (- pow2 15) (sint_v y);
+    assert(- sint_v x * (- pow2 15) <= sint_v x * sint_v y /\ sint_v x * sint_v y <= - sint_v x * pow2 15);
+    swap_neg_mul (- sint_v x) (pow2 15);
+    lemma_mult_le_right (pow2 15) (- pow2 15) (- sint_v x);
+    lemma_mult_le_right (pow2 15) (sint_v x) (pow2 15);
+    pow2_plus 15 15;
+    pow2_lt_compat 31 30;
+    assert(range (sint_v x * sint_v y) S32)
+    end
+
 let mul_m (x:montgomery_t) (y:montgomery_t) : Pure montgomery_t (requires True) (ensures fun r -> to_t r == Group.mul_t (to_t x) (to_t y)) =
-  assert_norm (range (sint_v x) S32);
-  assert_norm (range (sint_v y) S32);
-  assert_norm (sint_v x * sint_v y <= params_q * params_q);
-  assert_norm ( - params_q * params_q <= sint_v x * sint_v y);
-  assert_norm ( params_q * params_q < params_q * pow2 (params_logr-1));
-  assert_norm ( - params_q * pow2 (params_logr - 1) <= - params_q * params_q);
-  assert_norm ( params_q * params_q <= maxint S32);
-  assert_norm ( minint S32 <= - params_q * params_q);
-  assert (range (sint_v x * sint_v y) S32);
-  assert_norm ( - params_q * pow2 (params_logr-1) <= sint_v x * sint_v y /\ sint_v x * sint_v y < params_q * pow2 (params_logr -1));
+  assert_norm(-pow2 15 < - params_q);
+  mul_range_lemma_m x y;
   let mr () : GTot montgomery_t = montgomery_reduce_int32 ((to_i32 x) *! (to_i32 y)) in
   mul_lemma (to_i32 x) (to_i32 y);
   assert((sint_v (mr ()) * pow2 params_logr) % params_q = (sint_v x * sint_v y) % params_q);
@@ -87,6 +208,33 @@ let mul_m (x:montgomery_t) (y:montgomery_t) : Pure montgomery_t (requires True) 
   MGroup.lemma_equality1 (sint_v (mr ())) (SpecGroup.v (x' ()) * sint_v y);
   lemma_mod_mul_distr_r (SpecGroup.v (x' ())) (sint_v y) params_q;
   let y' () : GTot Group.t = to_t y in
+  let mr' () : GTot Group.t = to_t (mr ()) in
+  to_t_lemma y;
+  to_t_lemma (mr ());
+  lemma_mod_mul_distr_r (SpecGroup.v (x' ())) (SpecGroup.v (y' ()) * pow2 params_logr) params_q;
+  paren_mul_right (SpecGroup.v (x' ())) (SpecGroup.v (y' ())) (pow2 params_logr);
+  MGroup.lemma_equality1 (SpecGroup.v (mr' ())) (SpecGroup.v (x' ()) * SpecGroup.v (y' ()));
+  SpecGroup.mul_lemma_t (x' ()) (y' ());
+  modulo_lemma (SpecGroup.v (mr' ())) params_q;
+  montgomery_reduce_int32 ((to_i32 x) *! (to_i32 y))
+
+let mul_m_int16 (x:int16{sint_v x > pow2 15}) (y:montgomery_t) : Pure montgomery_t (requires True) (ensures fun r -> to_t r == Group.mul_t (int16_to_t x) (to_t y)) =
+  assert_norm(-pow2 15 < - params_q);
+  mul_range_lemma_m x y;
+  let mr () : GTot montgomery_t = montgomery_reduce_int32 ((to_i32 x) *! (to_i32 y)) in
+  mul_lemma (to_i32 x) (to_i32 y);
+  assert((sint_v (mr ()) * pow2 params_logr) % params_q = (sint_v x * sint_v y) % params_q);
+  lemma_mod_mul_distr_l (sint_v x) (sint_v y) params_q;
+  let x' () : GTot Group.t = int16_to_t x in
+  to_t_lemma x;
+  lemma_mod_mul_distr_l (SpecGroup.v (x' ()) * pow2 params_logr) (sint_v y) params_q;
+  paren_mul_right (SpecGroup.v (x' ())) (pow2 params_logr) (sint_v y);
+  swap_mul (pow2 params_logr) (sint_v y);
+  paren_mul_right (SpecGroup.v (x' ())) (sint_v y) (pow2 params_logr);
+  lemma_mod_mul_distr_l (SpecGroup.v (x' ()) * sint_v y) (pow2 params_logr) params_q;
+  MGroup.lemma_equality1 (sint_v (mr ())) (SpecGroup.v (x' ()) * sint_v y);
+  lemma_mod_mul_distr_r (SpecGroup.v (x' ())) (sint_v y) params_q;
+  let y' () : GTot Group.t = int16_to_t y in
   let mr' () : GTot Group.t = to_t (mr ()) in
   to_t_lemma y;
   to_t_lemma (mr ());
