code/kyber2/impl/Impl.Kyber2.Arithmetic.Sums.fsti
@@ -8,6 +8,7 @@ module MGroup = Impl.Kyber2.GroupMontgomery
 
 //open FStar.Tactics.Typeclasses
 open FStar.HyperStack.All
+open FStar.Mul
 
 open Kyber2.Params
 
@@ -27,6 +28,13 @@ val sum_n_montgomery:
   -> l:lbuffer (MGroup.montgomery_t) n
   -> output:lbuffer (MGroup.montgomery_t) (size 1)
   -> Stack unit (requires fun h -> live h l /\ live h output /\ Buf.disjoint l output) (ensures fun h0 _ h1 -> modifies1 output h0 h1 /\ MGroup.to_t (Seq.index h1.[|output|] 0) == Lib.Arithmetic.Sums.sum_n #Spec.Kyber2.Group.t #Spec.Kyber2.Group.monoid_plus_t (Seq.map MGroup.to_t h0.[|l|]))
+
+inline_for_extraction
+val sum_n_montgomery_no_plus_m:
+  #n:size_t{v n < pow2 (params_logr-1)}
+  -> l:lbuffer (MGroup.montgomery_t) n
+  -> output:lbuffer (x:int32{- params_q * pow2 (params_logr-1) <= sint_v x /\ sint_v x < params_q * pow2 (params_logr -1)}) (size 1)
+  -> Stack unit (requires fun h -> live h l /\ live h output /\ Buf.disjoint l output ) (ensures fun h0 _ h1 -> modifies1 output h0 h1 /\ (sint_v (Seq.index h1.[|output|] 0) >= - (v n) * params_q /\ sint_v (Seq.index h1.[|output|] 0) <= (v n) * params_q) /\ MGroup.int32_to_t (Seq.index h1.[|output|] 0) == Lib.Arithmetic.Sums.sum_n #Spec.Kyber2.Group.t #Spec.Kyber2.Group.monoid_plus_t (Seq.map MGroup.to_t h0.[|l|]))
 
 inline_for_extraction
 val sum_n_cbd:
